\begin{answer}

\[J(\theta) = -\frac{1}{\nexp} \sum_{i=1}^\nexp \left(y^{(i)}\log(h_{\theta}(x^{(i)})) +  (1 - y^{(i)})\log(1 - h_{\theta}(x^{(i)}))\right)\]
\[\frac{\partial J(\theta)}{\partial x_i} = \Sigma-(y - h(x)x_i\]
\[H_i_j =  \frac{\partial^2 J(\theta)}{\partial x^2}\] 
\[=\Sigma(\frac{\partial h(x)}{\partial \theta_j)}x_i  \]
\[=\Sigma (h(x)(1 - h(x)) x_jx_i \]
		Assume
\[x_ix_j = X_i_j \]  
\[=\Sigma (h(x)(1 - h(x)) xx^T\]

\[z^THz \geq 0\]
		is always positive-semidefinite when H \geq 0
		
\[z^THz =  z^T(\Sigma (h(x)(1 - h(x)) xx^T)z\]
\[=\Sigma (h(x)(1 - h(x)) (z^Txx^Tz)\]
\[=\Sigma (h(x)(1 - h(x)) (x^Tz)^2\]

\[(x^Tz)^2\]  
 		is positive, and \[h(x)(1 - h(x)\] 
 		is a bernoulli probability 
 where:
\[0 \leq h(x) \leq 1\] 
 Therefore, the value of that replaces the hessian determines whether $z^THz$  is positive semidefinite, or negative semidefinite. In this case the Hessian is positive semidefinite.
So, 
\[z^THz \geq 0\]

\end{answer}

