\begin{answer}


Given that:
\[p(y\vert x) = \frac{p(x\vert y) p(y)}{p(x)}\]
\[p(y = 1\vert x; \phi, \mu_0, \mu_1, \Sigma)
\[=\frac{p(x\vert y=1; \phi, \mu_0, \mu_1, \Sigma)p(y=1; \phi, \mu_0, \mu_1, \Sigma)}{p(x;\phi,\mu_0,\mu_1,\Sigma)}\]
\[=\frac{p(x\vert y=1)p(y=1)}{p(x)}\]
\[= \frac{p(x\vert y=1)p(y=1)}{p(x\vert y= 0)p(y=0)+p(x\vert y=1)p(y=1)}\]
\[=\frac{exp(\frac{-1}{2}(x-\mu_1)^T\Sigma^-1(x-\mu_1))(\phi)}{exp(\frac{-1}{2}(x-\mu_0)^T \Sigma^-1 (x-\mu_0))(1-\phi) + exp(\frac{-1}{2}(x-\mu_1)^T \Sigma^-1 (x-\mu_1))(\phi)}\]
\[= \frac{1}{1+\frac{1-\phi}{\phi}exp(\frac{-1}{2}(x-\mu_0)^T \Sigma^-1 (x-\mu_0) + \frac{1}{2}(x-\mu_1)^T \Sigma^-1 (x-\mu_1)}\]
\[=\frac{1}{1 + exp(\frac{-1}{2}((x-\mu_0)^T \Sigma^-1\mu_0 -\mu_1)^T \Sigma^-1 \mu_1) + log(\frac{1-\phi}{\phi}))}\]

rearranging terms
\[ (x - \mu_0)^T \Sigma^-1(x-\mu_0) - (x-\mu_1)^T \Sigma^-1(x-\mu_1) \]
\[= x^T\Sigma^-1 x - \mu_0^T \Sigma^-1 x - x^T \Sigma^-1 \mu_0 + \mu_0^T \Sigma^-1 \mu_0 - x^T \Sigma^-1 x + \mu_1^T \Sigma^-1 x + x^T \Sigma^-1 \mu_1 - \mu_1^T \Sigma^-1 \mu_1 \]
\[= -2 \mu_0^T \Sigma^-1 x + \mu_0^T \Sigma^-1 \mu_0 + 2 \mu_1^T \Sigma^-1 c - \mu_1^T \Sigma^-1 \mu_1 \]
\[= 2(\mu_1 - \mu_0)^T \Sigma^-1 x + \mu_0^T \Sigma^-1 \mu_0 - \mu_1^T \Sigma^-1 \mu_1 \]
Therefore: 
\[p(y = 1\vert x; \phi, \mu_0, \mu_1, \Sigma) = \[=\frac{1}{1 + exp(log \frac{1-\phi}{phi} + \frac{1}{2} \mu_1^T \Sigma^-1 \mu_1 - \frac{1}{2} \mu_0^T \Sigma^-1 \mu_0 + (\mu_0 - \mu_1)^T \Sigma^-1 x}\]
The term inside the exp can be expressed as a linear function
\[ \theta = \Sigma^-1 (\mu_1 - \mu_0) \]
\[ \theta_0 = \frac{1}{2}(\mu_0^T \Sigma^-1 \mu_0 - \mu_1 ^T \Sigma^-1 \mu_1) - log \frac{1-\phi}{\phi}
\end{answer}
