\begin{answer}

\centering
&&\text{the definition for the following observation} 
\[\ell_{semi-sup}(\theta) &=& \ell_{unsup}(\theta) + \alpha \ell_{sup}(\theta)  \]
\[&=& \sum_{i=1}^n  \sum_{z^(i)}  log p(x^{(i)} , z^{(i)}; \theta)} + \alpha \ell_{sup}(\theta^{(t+1)}) \]
&&\text{By Jensen's Inequality} 
\[&\geq& \sum_{i=1}^n  \sum_{z^(i)} Q_i^{(t)} (z^{(i)}) log \frac{p(x^{(i)} , z^{(i)}; \theta^{(t+1)})}{Q_i^{(t)} (z^{(i)} )} + \alpha \ell_{sup}(\theta^{(t+1)}) \]
&&\text{Under M-step} 
\[&\geq& \sum_{i=1}^n  \sum_{z^(i)} Q_i^{(t)} (z^{(i)}) log \frac{p(x^{(i)} , z^{(i)}; \theta)}{Q_i^{(t)} (z^{(i)} )} + \alpha \ell_{sup}(\theta^{(t)}) \]
\[&=& \ell_{unsup}(\theta^{(t)}) + \alpha \ell{sup}(\theta^{(t)}) \]
\[&=& \ell(\theta^{(t)}) \]

\end{answer}
