\begin{answer}

\begin{eqnarray*}
&&\hspace*{-63pt}\text{We have that} \\
w_j^{(i)} &=& p(z^{(i)} = j\mid x^{(i)} ; \phi, \mu, \Sigma)  \\
&=& \frac{p(x^{(i)} \mid z^{(i)} = j\mid x^{(i)} ; \phi, \mu, \Sigma) p(z^{(i)} = j; \theta)} {\sum_{l=1}^k p(x^{(i)} \mid z^{(i)} = l ;\mid x^{(i)} ; \phi, \mu, \Sigma) p(z^{(i)}  = l ; \theta)} \\
&=& \frac{ \frac{1} {\sqrt{(2\pi)^d\mid\Sigma_j\mid}} exp ( - \frac{1} {2} (x^{(i)} - \mu_j)^T \Sigma_j^{-1} (x^{(i)} -\mu_j))\phi_j } {\sum_{l=1}^k \frac{1} {\sqrt{(2\pi)^d\mid\Sigma_l\mid}} exp ( - \frac{1} {2} (x^{(i)} - \mu_l)^T \Sigma_l^{-1} (x^{(i)} -\mu_l))\phi_l} \\
&=& \frac{\mid\Sigma_j\mid^{-1} exp ( - \frac{1} {2} (x^{(i)} - \mu_j)^T \Sigma_j^{-1} (x^{(i)} -\mu_j))\phi_j } {\sum_{l=1}^k\mid\Sigma_l\mid^{-1} exp ( - \frac{1} {2} (x^{(i)} - \mu_l)^T \Sigma_l^{-1} (x^{(i)} -\mu_j))\phi_l }
\end{eqnarray*}

\end{answer}
