\begin{answer}

\begin{eqnarray*}
	The sum of probabilities for y given x is 1
	\[\int p(y\mid x; \theta)dy &=& 1\]
	Substituting for exponential family
	\[\int b(y)\exp(\eta^T y - a(\eta))dy &=& 1\]
	arranging equation
	\[\int b(y) \exp(\eta^T y)dy &=& exp(a(\eta))\]
	taking derivative w.r.t eta
	\[ \frac{\partial a(\eta}{\partial\eta} \int b(y) \exp(\eta^T y)dy &=& \frac{\partial a(\eta}{\partial\eta} exp(a(\eta))\]
	\[\int y b(y) \exp(\eta^T y)dy &=& \frac{\partial a(\eta}{\partial\eta} exp(a(\eta))\]
	Rearranging eq form 
	\[ \frac{\partial a(\eta}{\partial\eta} &=& \int y b(y)\exp(\eta^T y - a(\eta))dy &=& 1\] 
	additional term y, exp family probability form
	\[&=& \int y p(y\mid x; \theta) dy \]
	\[\frac{\partial a(\eta}{\partial\eta} &=& E[y\mid x: \theta] \]
\end{eqnarray*} 

\end{answer}
