\begin{answer}

\begin{eqnarray*}
\underset{\theta}{\operatorname{argmin}} K L (\hat{P} \| P_{\theta}) &=& \underset{\theta}{\operatorname{argmin}} \sum_x \hat{P}(x) \log \frac{\hat{P}(x)}{P_{\theta}(x)} \\
&=& \underset{\theta}{\operatorname{argmin}} \sum_x \hat{P}(x) \log \hat{P}(x) - \hat{P}(x) \log P_{\theta}(x)  \\
&=& \underset{\theta}{\operatorname{argmin}} \sum_x - \hat{P}(x) \log \frac{P_{\theta}(x)}{\hat{P}(x)} \\
&=& \underset{\theta}{\operatorname{argmax}} \sum_x \hat{P}(x) \log \frac{P_{\theta}(x)}{\hat{P}(x)} \\
&&\hspace*{-63pt}\text{We are given that $\hat{P}(x) = \frac{1}{n} \sum_{i=1}^n 1\{x^{(i)} = x\}$} \\
&=& \underset{\theta}{\operatorname{argmax}} \sum_x \frac{1}{n} \sum_{i=1}^n 1\{x^{(i)} = x\} \log \frac{P_{\theta} (x)}{\frac{1}{n} \sum 1\{x^{(i)} = x\} } \\
&=& \underset{\theta}{\operatorname{argmax}} \frac{1}{n} \sum_{i=1}^n \sum_x  1\{x^{(i)} = x\} \log P_{\theta}(x^{(i)})  \\
&=&\underset{\theta}{\operatorname{argmax}} \frac{1}{n} \sum_{i=1}^n \log P_{\theta}(x^{(i)}) \\
\underset{\theta}{\operatorname{argmin}} K L (\hat{P} \| P_{\theta}) &=& \underset{\theta}{\operatorname{argmax}} \sum_{i=1}^n \log P_{\theta}(x^{(i)}) \\
\end{eqnarray*}

\end{answer}
